Finish OnDecrypt refactoring
Everything verifies now, but need to deal with "compilation of seq<TRAIT> is not supported" now

src/StandardLibrary/StandardLibrary.dfy
@@ -391,4 +391,45 @@ module {:extern "STL"} StandardLibrary {
         assert LexicographicLessOrEqualAux(b, a, less, m);
     }
   }
+
+  // ----- foldl ----------
+
+  function method foldl<A,B>(f: (B,A) -> B, b: B, xs: seq<A>): B
+  {
+    if |xs| == 0 then
+      b
+    else 
+      foldl(f, f(b, xs[0]), xs[1..])
+  }
+
+  lemma SequenceCons<T>(xs: seq<T>) 
+      requires |xs| > 0
+      ensures [xs[0]] + xs[1..] == xs
+  {
+
+  }
+
+  // Here is FoldL_Property again, but this time with "f" instead of "stp".
+  lemma FoldL_Property_inv_f<A,B>(inv: (B,seq<A>) -> bool, f: (B,A) -> B, b: B, xs: seq<A>)
+    requires forall x, xs, b :: inv(b, [x] + xs) ==> inv(f(b, x), xs)
+    requires inv(b, xs)
+    ensures inv(foldl(f, b, xs), [])
+  {
+    // the rest of the calculation can be omitted.
+    if |xs| > 0 {
+      var head := xs[0];
+      var tail := xs[1..];
+      calc {
+        true;
+      ==>  // by the precondition
+        { SequenceCons(xs); }
+        inv(b, [head] + tail);  // TODO-RS: Need to prove property of seq + seq
+      ==>  // by the inductive property of "inv"
+        inv(f(b, head), tail);
+      ==>  { FoldL_Property_inv_f(inv, f, f(b, head), tail); }  // induction hypothesis
+        inv(foldl(f, f(b, head), tail), []);
+      }
+    }
+  }
+
 }
